Proved closure property of backtracker

correctness/RegexCorrectness/Backtracker/Traversal.lean
@@ -7,6 +7,7 @@ set_option autoImplicit false
 
 open Regex.Data (BitMatrix BoundedIterator)
 open String (Pos Iterator)
+open Regex.NFA (Step)
 
 namespace Regex.Backtracker.captureNextAux
 
@@ -296,6 +297,297 @@ theorem path_done_of_some {it₀} (hres : captureNextAux HistoryStrategy nfa wf 
         inv.reachable entry (by simp [mem])
       exact ⟨reachable⟩
     exact ih hres inv'
+
+end
+
+section
+
+variable {s : String} {nfa : NFA} {wf : nfa.WellFormed} {startIdx maxIdx : Nat} {visited : BitMatrix nfa.nodes.size (maxIdx + 1 - startIdx)} {stack : List (StackEntry HistoryStrategy nfa startIdx maxIdx)}
+
+structure StringInv (s : String) (stack : List (StackEntry HistoryStrategy nfa startIdx maxIdx)) where
+  eq : ∀ entry ∈ stack, entry.it.toString = s
+
+namespace StringInv
+
+theorem drop {entry} (inv : StringInv s (entry :: stack)) : StringInv s stack :=
+  ⟨fun entry' mem' => inv.eq entry' (by simp [mem'])⟩
+
+theorem cons {entry} (inv : StringInv s stack) (h : entry.it.toString = s) : StringInv s (entry :: stack) := by
+  refine ⟨fun entry' mem' => ?_⟩
+  simp at mem'
+  cases mem' with
+  | inl eq => rw [eq, h]
+  | inr mem' => exact inv.eq entry' mem'
+
+theorem cons_iff {entry} : StringInv s (entry :: stack) ↔ entry.it.toString = s ∧ StringInv s stack := by
+  apply Iff.intro
+  . intro inv
+    exact ⟨inv.eq entry (by simp), inv.drop⟩
+  . intro ⟨h, inv⟩
+    exact inv.cons h
+
+end StringInv
+
+structure ClosureInv (s : String) (visited : BitMatrix nfa.nodes.size (maxIdx + 1 - startIdx)) (stack : List (StackEntry HistoryStrategy nfa startIdx maxIdx)) where
+  step : ∀ (state : Fin nfa.nodes.size) (bit : BoundedIterator startIdx maxIdx) (state' : Fin nfa.nodes.size) (bit' : BoundedIterator startIdx maxIdx) (update : Option (Nat × Pos)),
+    bit.toString = s →
+    visited.get state bit.index →
+    nfa.Step 0 state bit.it state' bit'.it update →
+    visited.get state' bit'.index ∨ ∃ entry ∈ stack, entry.state = state' ∧ entry.it = bit'
+
+namespace ClosureInv
+
+theorem preserves {entry stack'} (inv : ClosureInv s visited (entry :: stack)) (hstring : entry.it.toString = s)
+  (nextEntries : List (StackEntry HistoryStrategy nfa startIdx maxIdx)) (hstack : stack' = nextEntries ++ stack)
+  (hnext : ∀ (state' : Fin nfa.nodes.size) (bit' : BoundedIterator startIdx maxIdx) (update : Option (Nat × Pos)),
+    nfa.Step 0 entry.state entry.it.it state' bit'.it update →
+    ∃ entry' ∈ nextEntries, entry'.state = state' ∧ entry'.it = bit') :
+  ClosureInv s (visited.set entry.state entry.it.index) stack' := by
+  refine ⟨?_⟩
+  intro state bit state' bit' update' eqs hmem step
+  simp [visited.get_set] at hmem
+  match hmem with
+  | .inl ⟨eqstate, eqindex⟩ =>
+    -- There is a step from the top entry. Use the given property to find the next entries in the next stack top.
+    have eqit : entry.it = bit := by
+      simp [BoundedIterator.ext_index_iff, eqindex, eqs, hstring]
+    have ⟨entry', hmem', eqstate', eqit'⟩ := hnext state' bit' update' (eqit ▸ eqstate ▸ step)
+    exact .inr ⟨entry', by simp [hstack, hmem'], eqstate', eqit'⟩
+  | .inr hmem =>
+    -- There is a step from the entry below the stack top.
+    match inv.step state bit state' bit' update' eqs hmem step with
+    | .inl hmem' => exact .inl (visited.get_set_of_get hmem')
+    | .inr ⟨entry', hmem', eqstate, eqit⟩ =>
+      simp at hmem'
+      cases hmem' with
+      | inl eq =>
+        -- If the step moves to the top entry, then this iteration marks the entry as visited.
+        simp [eq, ←eqstate, ←eqit, visited.get_set_eq]
+      | inr hmem' =>
+        -- If the step moves to the entry below the stack top, then the entry is still in the stack.
+        exact .inr ⟨entry', by simp [hstack, hmem'], eqstate, eqit⟩
+
+end ClosureInv
+
+/--
+When the backtracker returns `.none`, it explores all reachable states and thus the visited set satisfies the closure property under the step relation.
+-/
+theorem step_closure {s : String} {result} (hres : captureNextAux HistoryStrategy nfa wf startIdx maxIdx visited stack = result)
+  (isNone : result.1 = .none)
+  (cinv : ClosureInv s visited stack) (sinv : StringInv s stack) :
+  ClosureInv s result.2 [] := by
+  induction visited, stack using captureNextAux.induct' HistoryStrategy nfa wf startIdx maxIdx with
+  | base visited =>
+    simp [captureNextAux_base] at hres
+    simp [←hres, cinv]
+  | visited visited update state it stack' mem ih =>
+    simp [captureNextAux_visited mem] at hres
+    have cinv' : ClosureInv s visited stack' := by
+      refine ⟨?_⟩
+      intro state₁ bit state₂ bit' update' eqs hmem step
+      match cinv.step state₁ bit state₂ bit' update' eqs hmem step with
+      | .inl hmem' => exact .inl hmem'
+      | .inr ⟨entry, hmem', eqstate, eqit⟩ =>
+        simp at hmem'
+        cases hmem' with
+        | inl eq => simp [eq, ←eqstate, ←eqit, mem]
+        | inr hmem' => exact .inr ⟨entry, hmem', eqstate, eqit⟩
+    exact ih hres cinv' sinv.drop
+  | done visited update state it stack' mem hn =>
+    simp [captureNextAux_done mem hn] at hres
+    simp [←hres] at isNone
+  | fail visited update state it stack' mem visited' hn ih =>
+    rw [captureNextAux_fail mem hn] at hres
+    have cinv' : ClosureInv s visited' stack' := by
+      apply cinv.preserves (sinv.eq _ (by simp)) [] (by simp)
+      intro state' bit' update' step
+      rw [Step.iff_fail hn] at step
+      exact step.elim
+    exact ih hres cinv' sinv.drop
+  | epsilon visited update state it stack' mem visited' state' hn ih =>
+    rw [captureNextAux_epsilon mem hn] at hres
+    have cinv' : ClosureInv s visited' (⟨update, state', it⟩ :: stack') := by
+      apply cinv.preserves (sinv.eq _ (by simp)) [⟨update, state', it⟩] (by simp)
+      intro state'' bit'' update' step
+      rw [Step.iff_epsilon hn] at step
+      have ⟨_, eqstate'', eqit'', _⟩ := step
+      simp [Fin.eq_of_val_eq eqstate'', BoundedIterator.ext_iff, eqit'']
+    have sinv' : StringInv s (⟨update, state', it⟩ :: stack') := by
+      simp [StringInv.cons_iff, sinv.drop]
+      exact sinv.eq ⟨update, state, it⟩ (by simp)
+    exact ih hres cinv' sinv'
+  | split visited update state it stack' mem visited' state₁ state₂ hn ih =>
+    rw [captureNextAux_split mem hn] at hres
+    have cinv' : ClosureInv s visited' (⟨update, state₁, it⟩ :: ⟨update, state₂, it⟩ :: stack') := by
+      apply cinv.preserves (sinv.eq _ (by simp)) [⟨update, state₁, it⟩, ⟨update, state₂, it⟩] (by simp)
+      intro state'' bit'' update' step
+      rw [Step.iff_split hn] at step
+      have ⟨_, eqstate'', eqit'', _⟩ := step
+      simp [BoundedIterator.ext_iff, eqit'']
+      cases eqstate'' with
+      | inl eq₁ => simp [Fin.eq_of_val_eq eq₁]
+      | inr eq₂ => simp [Fin.eq_of_val_eq eq₂]
+    have sinv' : StringInv s (⟨update, state₁, it⟩ :: ⟨update, state₂, it⟩ :: stack') := by
+      simp [StringInv.cons_iff, sinv.drop]
+      exact sinv.eq ⟨update, state, it⟩ (by simp)
+    exact ih hres cinv' sinv'
+  | save visited update state it stack' mem visited' offset state' hn update' ih =>
+    rw [captureNextAux_save mem hn] at hres
+    have cinv' : ClosureInv s visited' (⟨update', state', it⟩ :: stack') := by
+      apply cinv.preserves (sinv.eq _ (by simp)) [⟨update', state', it⟩] (by simp)
+      intro state'' bit'' update' step
+      rw [Step.iff_save hn] at step
+      have ⟨_, eqstate'', eqit'', _⟩ := step
+      simp [Fin.eq_of_val_eq eqstate'', BoundedIterator.ext_iff, eqit'']
+    have sinv' : StringInv s (⟨update', state', it⟩ :: stack') := by
+      simp [StringInv.cons_iff, sinv.drop]
+      exact sinv.eq ⟨update, state, it⟩ (by simp)
+    exact ih hres cinv' sinv'
+  | anchor_pos visited update state it stack' mem visited' a state' hn ht ih =>
+    rw [captureNextAux_anchor_pos mem hn ht] at hres
+    have cinv' : ClosureInv s visited' (⟨update, state', it⟩ :: stack') := by
+      apply cinv.preserves (sinv.eq _ (by simp)) [⟨update, state', it⟩] (by simp)
+      intro state'' bit'' update' step
+      rw [Step.iff_anchor hn] at step
+      have ⟨_, eqstate'', eqit'', _⟩ := step
+      simp [Fin.eq_of_val_eq eqstate'', BoundedIterator.ext_iff, eqit'']
+    have sinv' : StringInv s (⟨update, state', it⟩ :: stack') := by
+      simp [StringInv.cons_iff, sinv.drop]
+      exact sinv.eq ⟨update, state, it⟩ (by simp)
+    exact ih hres cinv' sinv'
+  | anchor_neg visited update state it stack' mem visited' a state' hn ht ih =>
+    rw [captureNextAux_anchor_neg mem hn ht] at hres
+    have cinv' : ClosureInv s visited' stack' := by
+      apply cinv.preserves (sinv.eq _ (by simp)) [] (by simp)
+      intro state'' bit'' update' step
+      simp [Step.iff_anchor hn] at step
+      simp [step] at ht
+    exact ih hres cinv' sinv.drop
+  | char_pos visited update state it stack' mem visited' c state' hn hnext hc ih =>
+    rw [captureNextAux_char_pos mem hn hnext hc] at hres
+    have cinv' : ClosureInv s visited' (⟨update, state', it.next hnext⟩ :: stack') := by
+      apply cinv.preserves (sinv.eq _ (by simp)) [⟨update, state', it.next hnext⟩] (by simp)
+      intro state'' bit'' update' step
+      rw [Step.iff_char hn] at step
+      have ⟨l, r, _, eqstate'', eqit'', _, _⟩ := step
+      simp [Fin.eq_of_val_eq eqstate'', BoundedIterator.ext_iff, eqit'', BoundedIterator.next, Iterator.next'_eq_next]
+    have sinv' : StringInv s (⟨update, state', it.next hnext⟩ :: stack') := by
+      simp [StringInv.cons_iff, BoundedIterator.next_toString, sinv.drop]
+      exact sinv.eq ⟨update, state, it⟩ (by simp)
+    exact ih hres cinv' sinv'
+  | char_neg visited update state it stack' mem visited' c state' hn hnext hc ih =>
+    rw [captureNextAux_char_neg mem hn hnext hc] at hres
+    have cinv' : ClosureInv s visited' stack' := by
+      apply cinv.preserves (sinv.eq _ (by simp)) [] (by simp)
+      intro state'' bit'' update' step
+      rw [Step.iff_char hn] at step
+      have ⟨l, r, _, _, _, _, vf⟩ := step
+      simp at vf
+      simp [BoundedIterator.curr, Iterator.curr'_eq_curr, vf.curr] at hc
+    exact ih hres cinv' sinv.drop
+  | char_end visited update state it stack' mem visited' c state' hn hnext ih =>
+    rw [captureNextAux_char_end mem hn hnext] at hres
+    have cinv' : ClosureInv s visited' stack' := by
+      apply cinv.preserves (sinv.eq _ (by simp)) [] (by simp)
+      intro state'' bit'' update' step
+      rw [Step.iff_char hn] at step
+      have ⟨l, r, _, _, _, _, vf⟩ := step
+      simp at vf
+      simp [BoundedIterator.hasNext, vf.hasNext] at hnext
+    exact ih hres cinv' sinv.drop
+  | sparse_pos visited update state it stack' mem visited' cs state' hn hnext hc ih =>
+    rw [captureNextAux_sparse_pos mem hn hnext hc] at hres
+    have cinv' : ClosureInv s visited' (⟨update, state', it.next hnext⟩ :: stack') := by
+      apply cinv.preserves (sinv.eq _ (by simp)) [⟨update, state', it.next hnext⟩] (by simp)
+      intro state'' bit'' update' step
+      rw [Step.iff_sparse hn] at step
+      have ⟨l, c, r, _, eqstate'', eqit'', _, vf, hc'⟩ := step
+      simp [Fin.eq_of_val_eq eqstate'', BoundedIterator.ext_iff, eqit'', BoundedIterator.next, Iterator.next'_eq_next]
+    have sinv' : StringInv s (⟨update, state', it.next hnext⟩ :: stack') := by
+      simp [StringInv.cons_iff, BoundedIterator.next_toString, sinv.drop]
+      exact sinv.eq ⟨update, state, it⟩ (by simp)
+    exact ih hres cinv' sinv'
+  | sparse_neg visited update state it stack' mem visited' cs state' hn hnext hc ih =>
+    rw [captureNextAux_sparse_neg mem hn hnext hc] at hres
+    have cinv' : ClosureInv s visited' stack' := by
+      apply cinv.preserves (sinv.eq _ (by simp)) [] (by simp)
+      intro state'' bit'' update' step
+      rw [Step.iff_sparse hn] at step
+      have ⟨l, c, r, _, _, _, _, vf, hc'⟩ := step
+      simp at vf
+      simp [BoundedIterator.curr, Iterator.curr'_eq_curr, vf.curr] at hc
+      exact (hc hc').elim
+    exact ih hres cinv' sinv.drop
+  | sparse_end visited update state it stack' mem visited' cs state' hn hnext ih =>
+    rw [captureNextAux_sparse_end mem hn hnext] at hres
+    have cinv' : ClosureInv s visited' stack' := by
+      apply cinv.preserves (sinv.eq _ (by simp)) [] (by simp)
+      intro state'' bit'' update' step
+      rw [Step.iff_sparse hn] at step
+      have ⟨l, c, r, _, _, _, _, vf, _⟩ := step
+      simp at vf
+      simp [BoundedIterator.hasNext, vf.hasNext] at hnext
+    exact ih hres cinv' sinv.drop
+
+def StepClosure (s : String) (visited : BitMatrix nfa.nodes.size (maxIdx + 1 - startIdx)) : Prop :=
+  ∀ (state : Fin nfa.nodes.size) (bit : BoundedIterator startIdx maxIdx) (state' : Fin nfa.nodes.size) (bit' : BoundedIterator startIdx maxIdx) (update : Option (Nat × Pos)),
+    bit.toString = s →
+    visited.get state bit.index →
+    nfa.Step 0 state bit.it state' bit'.it update →
+    visited.get state' bit'.index
+
+def PathClosure (s : String) (visited : BitMatrix nfa.nodes.size (maxIdx + 1 - startIdx)) : Prop :=
+  ∀ (state : Fin nfa.nodes.size) (bit : BoundedIterator startIdx maxIdx) (state' : Fin nfa.nodes.size) (bit' : BoundedIterator startIdx maxIdx) (update : List (Nat × Pos)),
+    bit.toString = s →
+    visited.get state bit.index →
+    nfa.Path 0 state bit.it state' bit'.it update →
+    visited.get state' bit'.index
+
+theorem PathClosure.of_step_closure {s} (wf : nfa.WellFormed) (h : StepClosure s visited) : PathClosure s visited := by
+  let motive (i : Nat) (it : Iterator) : Prop :=
+    ∃ (isLt : i < nfa.nodes.size) (bit : BoundedIterator startIdx maxIdx), bit.toString = s ∧ it = bit.it ∧ visited.get ⟨i, isLt⟩ bit.index
+  have cls i it j it' update (base : motive i it) (step : nfa.Step 0 i it j it' update) : motive j it' := by
+    have ⟨_, bit, eqs, eqit, hmem⟩ := base
+
+    have ge' : startIdx ≤ it'.pos.byteIdx :=
+      calc startIdx
+        _ ≤ it.pos.byteIdx := eqit ▸ bit.ge
+        _ ≤ it'.pos.byteIdx := step.le_pos
+    have le' : it'.pos.byteIdx ≤ maxIdx :=
+      calc it'.pos.byteIdx
+        _ ≤ it.toString.endPos.byteIdx := step.le_endPos
+        _ = maxIdx := eqit ▸ bit.eq.symm
+    have eq' : maxIdx = it'.toString.endPos.byteIdx :=
+      calc maxIdx
+        _ = it.toString.endPos.byteIdx := eqit ▸ bit.eq
+        _ = it'.toString.endPos.byteIdx := by rw [step.toString_eq]
+    let bit' : BoundedIterator startIdx maxIdx := ⟨it', ge', le', eq'⟩
+
+    have eqs' : bit'.toString = s := by
+      simpa [bit', BoundedIterator.toString, ←eqs, ←eqit] using step.toString_eq
+    have visited' := h ⟨i, step.lt⟩ bit ⟨j, step.lt_right wf⟩ bit' update eqs hmem (by simp [←eqit, bit', step])
+    exact ⟨step.lt_right wf, bit', eqs', rfl, visited'⟩
+
+  intro state bit state' bit' update eqs hmem path
+  have ⟨isLt, _, eqs, eqit, hmem'⟩ := path.of_step_closure motive cls ⟨state.isLt, bit, eqs, rfl, hmem⟩
+  exact (BoundedIterator.ext eqit) ▸ hmem'
+
+/--
+The closure property of the visited set can be lifted to paths.
+
+Note: `nfa.Path` requires at least one step, so this is a transitive closure. However, the existence in the visited set
+is obviously reflexive.
+-/
+theorem path_closure {s} {result} (hres : captureNextAux HistoryStrategy nfa wf startIdx maxIdx visited stack = result)
+  (isNone : result.1 = .none)
+  (cinv : ClosureInv s visited stack) (sinv : StringInv s stack) :
+  PathClosure s result.2 := by
+  have cinv' : ClosureInv s result.2 [] := step_closure hres isNone cinv sinv
+  have step_closure : StepClosure s result.2 := by
+    intro state bit state' bit' update eqs hmem step
+    have := cinv'.step state bit state' bit' update eqs hmem step
+    simpa
+  exact PathClosure.of_step_closure wf step_closure
 
 end
 
